Safe malloc - WIP

theories/examples/safe_malloc.v
@@ -37,8 +37,8 @@ Section SimpleMalloc.
 
   (* TODO we actually NEED to store the capability pointing to the lock,
           because we only have the RX permission, not RWX. *)
-  (* offset_lock = last address of the free memory *)
-  Definition malloc_pre_spin (offset_lock : Z) :=
+  (* offset_lock -> bmid *)
+  Definition malloc_pre_spin (offset : Z) :=
     encodeInstrsW [
         (* bm: *)
      Lt r_t3 0 r_t1; (* ;; check that size > 0 *)
@@ -48,14 +48,14 @@ Section SimpleMalloc.
      Fail;
         (* xm: *)
      Mov r_t5 PC;
-     Lea r_t5 (offset_lock - 5)%Z;
+     Lea r_t5 (offset - 5)%Z;
      Load r_t5 r_t5
       ].
 
-  Definition malloc_post_spin (offset : Z) :=
+  Definition malloc_post_spin (offset: Z) :=
     encodeInstrsW [
      Mov r_t2 PC;
-     Lea r_t2 offset;
+     Lea r_t2 (offset +2)%Z;
      (* ;; r2 = (RWX, bm, em, bmid) *)
      Load r_t2 r_t2;  (* ;; r2 = (RWX, bmid, em, a)  *)
      GetA r_t3 r_t2;
@@ -70,10 +70,14 @@ Section SimpleMalloc.
      Sub r_t1 0%Z r_t1;
      Lea r_t3 r_t1;
      GetB r_t1 r_t3;
+     Add r_t1 r_t1 2;
      Lea r_t3 r_t1;   (* ;; r3 = (RWX, bmid, em, bmid)       *)
      Store r_t3 r_t2; (* ;; bmid <- (RWX, bmid, em, a+size)  *)
-     Mov r_t1 r_t4;   (* ;; r3 = (RWX, a, a+size, a)         *)
-     Store r_t5 0;    (* Release the lock - we don't need CAS *)
+     Mov r_t1 r_t4   (* ;; r3 = (RWX, a, a+size, a)         *)
+     ].
+
+  Definition malloc_clear  :=
+    encodeInstrsW [
      Mov r_t2 0%Z;    (* Clear the registers *)
      Mov r_t3 0%Z;
      Mov r_t4 0%Z;
@@ -91,68 +95,85 @@ Section SimpleMalloc.
       ].
 
 
-  Definition malloc_subroutine_instrs' (offset offset_lock: Z) :=
-     malloc_pre_spin offset_lock
-       ++ spinlock_instrs' r_t5 r_t6 r_t7 r_t8
-       ++ malloc_post_spin offset.
-
-  Definition malloc_pre_spin_length : Z :=
+  Definition malloc_pre_length : Z :=
     Eval cbv in (length (malloc_pre_spin 0%Z)).
 
-  Definition malloc_pre_post_length : Z :=
-    Eval cbv in (length (malloc_pre_spin 0%Z)).
+  Definition malloc_post_length : Z :=
+    Eval cbv in (length (malloc_post_spin 0%Z)).
 
-  Definition spinlock_length : Z :=
-    Eval cbv in (length (spinlock_instrs' PC PC PC PC)).
+  Definition malloc_clear_length : Z :=
+    Eval cbv in (length (malloc_post_spin 0%Z)).
+
+  Definition malloc_subroutine_instrs' (offset_bmid : Z) :=
+     malloc_pre_spin offset_bmid
+       ++ acquire_spinlock_instrs r_t5 r_t6 r_t7 r_t8
+       ++ malloc_post_spin (offset_bmid - malloc_pre_length - acquire_spinlock_length)
+       ++ release_spinlock_instrs r_t5
+       ++ malloc_clear.
 
   Definition malloc_subroutine_instrs_length : Z :=
-    Eval cbv in (length (malloc_subroutine_instrs' 0%Z 0%Z)).
+    Eval cbv in (length (malloc_subroutine_instrs' 0%Z)).
+
+  Definition offset_bm : Z :=
+    Eval cbv in (malloc_subroutine_instrs_length).
 
   Definition malloc_subroutine_instrs (offset_lock : Z) :=
-    malloc_subroutine_instrs'
-      (malloc_subroutine_instrs_length - (5+spinlock_length))
-      offset_lock.
+    malloc_subroutine_instrs' offset_bm.
+
+
+
+
 
   Definition malloc_inv (b e : Addr) γ : iProp Σ :=
+    let b_m := (b ^+ malloc_subroutine_instrs_length)%a in
     (codefrag b (malloc_subroutine_instrs e)
-     ∗ e ↦ₐ WCap RWX b (e^+2)%a (e^+1)%a
-     ∗ is_lock γ (e ^+1)%a
-         (  ∃ b_m a_m,
-             ⌜(b + malloc_subroutine_instrs_length)%a = Some b_m⌝
-             ∗ b_m ↦ₐ (WCap RWX b_m e a_m)
+     ∗ b_m ↦ₐ WCap RWX b e (b_m ^+1)%a
+     ∗ ⌜(b + malloc_subroutine_instrs_length)%a = Some b_m⌝
+     ∗ is_lock γ (b_m ^+1)%a
+         (  ∃ a_m,
+               (b_m ^+ 2)%a ↦ₐ (WCap RWX b_m e a_m)
              ∗ [[a_m, e]] ↦ₐ [[ region_addrs_zeroes a_m e ]]
-             ∗ ⌜(b_m < a_m)%a ∧ (a_m <= e)%a⌝)%I).
+             ∗ ⌜((b_m ^+2)%a < a_m)%a ∧ (a_m <= e)%a⌝)%I).
+
+
+
+
 
 
   Lemma malloc_prelock_spec
     (i : CoreN)
     (wsize: Word)
-    (b e : Addr)
+    (b e b_m a_pre: Addr)
     w2 w3 w5
     N E
     (φ : language.val cap_lang → iProp Σ) :
 
-    let e' := (e^+2)%a in
-    SubBounds b e' b (b ^+ malloc_subroutine_instrs_length)%a ->
+    let e_pre := (a_pre ^+ malloc_pre_length)%a in
+    (b + malloc_subroutine_instrs_length)%a = Some b_m ->
+    b = a_pre ->
+    SubBounds b e a_pre e_pre ->
+
     ↑N ⊆ E →
-    (    inv N (codefrag b (malloc_pre_spin e)
-                ∗ e ↦ₐ WCap RWX b e' (e^+1)%a)
-         ∗ (i, PC) ↦ᵣ WCap RX b e' b
+    (    inv N (codefrag a_pre (malloc_pre_spin offset_bm)
+                ∗ b_m ↦ₐ WCap RWX b e (b_m^+1)%a)
+         ∗ (i, PC) ↦ᵣ WCap RX b e a_pre
          ∗ (i, r_t1) ↦ᵣ wsize
          ∗ (i, r_t2) ↦ᵣ w2
          ∗ (i, r_t3) ↦ᵣ w3
          ∗ (i, r_t5) ↦ᵣ w5
-         ∗ ▷ (   (i, PC) ↦ᵣ WCap RX b e' (b ^+ malloc_pre_spin_length)%a
+         ∗ ▷ (   (i, PC) ↦ᵣ WCap RX b e e_pre
                  ∗ (i, r_t1) ↦ᵣ wsize
-                 ∗ (i, r_t2) ↦ᵣ WCap RX b e' (b ^+ 5)%a
+                 ∗ (i, r_t2) ↦ᵣ WCap RX b e (a_pre ^+ 5)%a
                  ∗ (i, r_t3) ↦ᵣ WInt 1%nat
-                 ∗ (i, r_t5) ↦ᵣ WCap RWX b e' (e ^+1)%a
+                 ∗ (i, r_t5) ↦ᵣ WCap RWX b e (b_m ^+ 1)%a
                  ∗ ⌜ exists size:Z, (0 < size)%Z /\ wsize = WInt size ⌝
                  -∗ WP (i, Seq (Instr Executable)) @ E {{ φ }}%I))
     ⊢ WP (i, Seq (Instr Executable)) @ E {{ λ v, φ v ∨ ⌜v = (i, FailedV)⌝ }}%I.
   Proof.
-    intro e'.
-    iIntros (Hbounds HN) "(#Hfinv & HPC & Hr1 & Hr2 & Hr3 & Hr5 & Hφ)".
+    intro e_pre.
+    subst e_pre.
+    rewrite /malloc_pre_length.
+    iIntros (Hbm -> Hbounds HN) "(#Hfinv & HPC & Hr1 & Hr2 & Hr3 & Hr5 & Hφ)".
     iDestruct (inv_split_l with "Hfinv") as "Hinv".
     destruct (wsize) as [size|].
 
@@ -171,7 +192,9 @@ Section SimpleMalloc.
 
 
     do 3 iInstr_inv "Hinv".
-    { transitivity (Some e). admit. done. }
+    { transitivity (Some b_m). rewrite /malloc_subroutine_instrs_length in Hbm.
+      rewrite /offset_bm.
+      solve_addr. done. }
 
     wp_instr
     ; iInv "Hfinv" as ">[Hprog Hcaplock]" "Hcls"
@@ -180,10 +203,10 @@ Section SimpleMalloc.
     iApply ( wp_load_success_same_notinstr with "[$HPC $Hi $Hr5 $Hcaplock]").
     { exact (WInt 0). } (* TODO : why do I have to provide a word ? *)
     { rewrite decode_encode_instrW_inv ; auto. }
-    { apply isCorrectPC_intro; [admit| auto]. }
+    { apply isCorrectPC_intro; [solve_addr| auto]. }
     { auto. }
     { admit. }
-    { transitivity (Some (b ^+8)%a) ; solve_addr ; done. }
+    { transitivity (Some (a_pre ^+8)%a) ; solve_addr ; done. }
     iNext ; iIntros "(HPC & Hr5 & Hi & Hcaplock)".
     iDestruct ("Hcont" with "Hi") as "Hprog".
     iMod ("Hcls" with "[$Hprog $Hcaplock]") as "_".
@@ -191,13 +214,256 @@ Section SimpleMalloc.
 
     iApply (wp_wand with "[-]").
     { iApply "Hφ".
-      rewrite /malloc_pre_spin_length.
+      rewrite /malloc_pre_length.
       iFrame.
       iPureIntro. eexists. split ; eauto. }
     iIntros (?) "?" ; iFrame.
   Admitted.
 
-  
+  (* TODO move somewhere else *)
+  Tactic Notation "solve_length_seq" "by" tactic3(solve_a) :=
+    cbn ; try (rewrite finz_seq_between_length)
+    ; repeat (rewrite finz_dist_S ; last solve_a)
+    ; by rewrite finz_dist_0 ; last solve_a.
+
+  Ltac solve_dist_finz :=
+    match goal with
+    | h: _ |- ?n = finz.dist _ _
+      => symmetry
+    end
+    ; match goal with
+      | h: _ |- finz.dist ?b (?b^+?n)%a = ?n' =>
+          let H := fresh in
+          assert (H : (b+n)%f = Some (b ^+ n)%a) by solve_addr
+          ; apply (finz_incr_iff_dist b (b ^+n)%a n') in H
+          ; destruct H as [_ H] ; apply H
+      end.
+
+
+  Lemma malloc_postlock_spec
+    (i : CoreN)
+    (size: Z)
+    (b e e' a_post a_m : Addr)
+    w2 w3 w4
+    N E
+    (φ : language.val cap_lang → iProp Σ) :
+
+    let e_post := (a_post ^+ malloc_post_length)%a in
+    let b_m := (b ^+ (malloc_subroutine_instrs_length))%a in
+    a_post = (b ^+ malloc_pre_length ^+ acquire_spinlock_length)%a ->
+
+    SubBounds b e a_post e_post ->
+    ↑N ⊆ E →
+    (    inv N (codefrag a_post (malloc_post_spin (offset_bm - malloc_pre_length - acquire_spinlock_length)))
+         ∗ (i, PC) ↦ᵣ WCap RX b e a_post
+         ∗ (i, r_t1) ↦ᵣ WInt size
+         ∗ (i, r_t2) ↦ᵣ w2
+         ∗ (i, r_t3) ↦ᵣ w3
+         ∗ (i, r_t4) ↦ᵣ w4
+         ∗ (b_m ^+ 2)%a ↦ₐ WCap RWX b_m e' a_m
+         ∗ ▷ (   (i, PC) ↦ᵣ WCap RX b e (a_post ^+ malloc_post_length)%a
+                 ∗ (i, r_t1) ↦ᵣ WCap RWX a_m (a_m ^+ size)%a a_m
+                 ∗ (i, r_t2) ↦ᵣ WCap RWX b_m e' (a_m ^+ size)%a
+                 ∗ (i, r_t3) ↦ᵣ WCap RWX b_m e' (b_m ^+ 2)%a
+                 ∗ (i, r_t4) ↦ᵣ WCap RWX a_m (a_m ^+ size)%a a_m
+                 ∗ (b_m ^+ 2)%a ↦ₐ WCap RWX b_m e' (a_m ^+ size)%a
+                 ∗ ⌜ exists am', (a_m ^+ size)%a = am' /\ isWithin a_m am' (b ^+ malloc_subroutine_instrs_length)%a e = true⌝
+                 -∗ WP (i, Seq (Instr Executable)) @ E {{ φ }}%I))
+    ⊢ WP (i, Seq (Instr Executable)) @ E {{ λ v, φ v ∨ ⌜v = (i, FailedV)⌝ }}%I.
+  Proof.
+    intros e_post b_m.
+    iIntros ( -> Hbounds HN) "(#Hinv & HPC & Hr1 & Hr2 & Hr3 & Hr4 & Hb_m & Hφ)".
+    iInstr_inv "Hinv".
+    iInstr_inv "Hinv".
+    { rewrite /offset_bm /malloc_pre_length /acquire_spinlock_length.
+      transitivity (Some (b ^+ 43)%a). admit. done. }
+    subst b_m.
+    replace ((b ^+ malloc_subroutine_instrs_length) ^+ 2)%a
+      with ( b ^+ 43 )%a
+           by (rewrite /malloc_subroutine_instrs_length ; solve_addr).
+
+
+    iInstr_inv "Hinv".
+    admit.
+    iInstr_inv "Hinv".
+
+    (* Lea might fail *)
+    (* Lea *)
+    (* Open the invariant *)
+    wp_instr
+    ; iInv "Hinv" as ">Hprog" "Hcls"
+    (* Apply the invariant *)
+    ; iInstr_lookup "Hprog" as "Hi" "Hcont".
+
+    destruct (a_m + size)%a as [a_m'|] eqn:Ha_m'; cycle 1.
+    { (* Failure case: no registered rule for that yet; do it the manual way *)
+      (* TODO: cf malloc, do not use rmap, but an empty map *)
+      iAssert ([∗ map] k↦x ∈ (∅:gmap (CoreN * RegName) Word), k ↦ᵣ x)%I as "-#Hregs".
+        by rewrite big_sepM_empty.
+
+      iDestruct (big_sepM_insert with "[$Hregs $Hr2]") as "Hregs".
+      by rewrite lookup_empty.
+      iDestruct (big_sepM_insert with "[$Hregs $Hr1]") as "Hregs".
+      rewrite !lookup_insert_ne
+      ; first by rewrite lookup_empty.
+      all: try (match goal with
+                | h:_ |- _ ≠ _ => simplify_pair_eq
+                end).
+      iDestruct (big_sepM_insert with "[$Hregs $HPC]") as "Hregs".
+      rewrite !lookup_insert_ne
+      ; first by rewrite lookup_empty.
+      all: try (match goal with
+                | h:_ |- _ ≠ _ => simplify_pair_eq
+                end).
+
+      iApply (wp_lea _ i RX b e (((b ^+ malloc_pre_length) ^+ acquire_spinlock_length) ^+ 4)%a
+               with "[$Hregs $Hi]").
+      { rewrite decode_encode_instrW_inv; done. }
+      { admit. }
+      { apply lookup_insert. }
+      { rewrite /regs_of_core !dom_insert_L dom_empty_L. set_solver-. }
+      iNext. iIntros (regs' retv) "(Hspec & Hi & ?)".
+      iDestruct "Hspec" as %Hspec.
+
+      iDestruct ("Hcont" with "Hi") as "Hprog".
+      iMod ("Hcls" with "Hprog") as "_".
+
+      destruct Hspec as [| Hfail].
+      { exfalso.
+        clear - H4 Ha_m' H7 H6.
+        simplify_map_eq by simplify_pair_eq. }
+      { cbn.
+        iApply wp_pure_step_later; auto.
+        do 2 iModIntro.
+        iApply wp_value.
+        auto. } }
+
+    iApply ( wp_lea_success_reg with "[ $HPC $Hr2 $Hr1 $Hi ]") ; eauto.
+    { cbn ;rewrite decode_encode_instr_inv; eauto. }
+    { admit. }
+    { transitivity (Some (((b ^+ malloc_pre_length) ^+ acquire_spinlock_length) ^+ 5)%a); solve_addr; done. }
+    iNext; iIntros "(HPC & Hi & Hr1 & Hr2)".
+    (* Close the invariant *)
+    iDestruct ("Hcont" with "Hi") as "Hprog".
+    iMod ("Hcls" with "Hprog") as "_".
+    simpl ; iModIntro ; wp_pure.
+
+    iInstr_inv "Hinv".
+    iInstr_inv "Hinv".
+
+
+    (* might fail *)
+    (* subseg *)
+    (* Open the invariant *)
+    wp_instr
+    ; iInv "Hinv" as ">Hprog" "Hcls"
+    (* Apply the invariant *)
+    ; iInstr_lookup "Hprog" as "Hi" "Hcont".
+
+    destruct (isWithin a_m a_m' (b ^+ malloc_subroutine_instrs_length)%a e) eqn:Ha_m'_within; cycle 1.
+    { (* Failure case: manual mode. *)
+      iAssert ([∗ map] k↦x ∈ (∅:gmap (CoreN * RegName) Word), k ↦ᵣ x)%I as "-#Hregs".
+        by rewrite big_sepM_empty.
+
+      iDestruct (big_sepM_insert with "[$Hregs $Hr4]") as "Hregs".
+      by rewrite lookup_empty.
+      iDestruct (big_sepM_insert with "[$Hregs $Hr3]") as "Hregs".
+      rewrite !lookup_insert_ne
+      ; first by rewrite lookup_empty.
+      all: try (match goal with
+                | h:_ |- _ ≠ _ => simplify_pair_eq
+                end).
+      iDestruct (big_sepM_insert with "[$Hregs $Hr1]") as "Hregs".
+      rewrite !lookup_insert_ne
+      ; first by rewrite lookup_empty.
+      all: try (match goal with
+                | h:_ |- _ ≠ _ => simplify_pair_eq
+                end).
+      iDestruct (big_sepM_insert with "[$Hregs $HPC]") as "Hregs".
+      rewrite !lookup_insert_ne
+      ; first by rewrite lookup_empty.
+      all: try (match goal with
+                | h:_ |- _ ≠ _ => simplify_pair_eq
+                end).
+
+      iApply (wp_Subseg with "[$Hregs $Hi]").
+      { rewrite decode_encode_instrW_inv; done. }
+      { admit. }
+      { apply lookup_insert. }
+      { rewrite /regs_of_core !dom_insert_L dom_empty_L. set_solver-. }
+      iNext. iIntros (regs' retv) "(Hspec & Hi & ?)".
+
+      iDestruct ("Hcont" with "Hi") as "Hprog".
+      iMod ("Hcls" with "Hprog") as "_".
+
+      iDestruct "Hspec" as %Hspec.
+      destruct Hspec as [| Hfail].
+      { exfalso. unfold addr_of_argument in *.
+        (* clear -H6 H8 H9 H10 Ha_m'_within Ha_m'. *)
+        simplify_map_eq by simplify_pair_eq.
+        repeat match goal with H:_ |- _ => apply finz_of_z_eq_inv in H end; subst.
+        admit. }
+        (* congruence. } *)
+      { cbn. iModIntro. wp_pure. wp_end. auto. } }
+
+    iApply ( wp_subseg_success with "[ $HPC $Hr4 $Hr3 $Hr1 $Hi ]") ; eauto.
+    { cbn ;rewrite decode_encode_instr_inv; eauto. }
+    { admit. }
+    { transitivity (Some a_m); solve_addr; done. }
+    { transitivity (Some (a_m ^+ size)%a); solve_addr; done. }
+    { admit. }
+    { transitivity (Some (((b ^+ malloc_pre_length) ^+ acquire_spinlock_length) ^+ 8)%a); solve_addr; done. }
+    iNext; iIntros "(HPC & Hi & Hr3 & Hr1 & Hr4)".
+    (* Close the invariant *)
+    iDestruct ("Hcont" with "Hi") as "Hprog".
+    iMod ("Hcls" with "Hprog") as "_".
+    simpl ; iModIntro ; wp_pure.
+
+
+    iInstr_inv "Hinv".
+    iInstr_inv "Hinv".
+    { transitivity (Some a_m); solve_addr; done. }
+    iInstr_inv "Hinv".
+    iInstr_inv "Hinv".
+    iInstr_inv "Hinv".
+    { transitivity (Some 0%a); solve_addr; done. }
+    iInstr_inv "Hinv".
+    iInstr_inv "Hinv".
+
+    (* Lea *)
+    (* Open the invariant *)
+    wp_instr
+    ; iInv "Hinv" as ">Hprog" "Hcls"
+    (* Apply the invariant *)
+    ; iInstr_lookup "Hprog" as "Hi" "Hcont".
+    iApply ( wp_lea_success_reg with "[ $HPC $Hr3 $Hr1 $Hi ]") ; eauto.
+    { cbn ;rewrite decode_encode_instr_inv; eauto. }
+    { admit. }
+    { transitivity (Some (( (b ^+ malloc_pre_length) ^+ acquire_spinlock_length)^+16)%a); solve_addr; done. }
+    { transitivity (Some ((b ^+ 43)%a))
+      ; rewrite /malloc_subroutine_instrs_length. admit. done. }
+    iNext; iIntros "(HPC & Hi & Hr1 & Hr3)".
+    (* Close the invariant *)
+    iDestruct ("Hcont" with "Hi") as "Hprog".
+    iMod ("Hcls" with "Hprog") as "_".
+    simpl ; iModIntro ; wp_pure.
+
+
+
+    iInstr_inv "Hinv".
+    { admit. }
+    iInstr_inv "Hinv".
+
+
+    iApply (wp_wand with "[-]").
+    { iApply "Hφ".
+      replace a_m' with (a_m ^+ size)%a by solve_addr.
+      iFrame. iPureIntro ; eexists a_m' ; split ; eauto ; solve_addr.
+    }
+    iIntros (?) "?" ; iFrame.
+  Admitted.
+
+
   Lemma simple_malloc_subroutine_spec
     (i : CoreN)
     (wsize: Word)
@@ -210,12 +476,12 @@ Section SimpleMalloc.
     dom (gset (CoreN*RegName)) rmap =
       (set_map (fun r => (i,r)) all_registers_s) ∖ {[ (i, PC); (i, r_t0) ; (i, r_t1) ]} →
 
-    (exists b_m, (b + malloc_subroutine_instrs_length)%a = Some b_m /\ (b_m < e)%a) ->
+    (exists b_m, (b + malloc_subroutine_instrs_length)%a = Some b_m /\ ((b_m ^+ 2)%a < e)%a) ->
     ↑N ⊆ E →
     (  inv N (malloc_inv b e γ)
      ∗ ([∗ map] r↦w ∈ rmap, r ↦ᵣ w)
      ∗ (i, r_t0) ↦ᵣ cont
-     ∗ (i, PC) ↦ᵣ WCap RX b (e ^+2)%a b
+     ∗ (i, PC) ↦ᵣ WCap RX b e b
      ∗ (i, r_t1) ↦ᵣ wsize
        ∗ ▷ (([∗ map] r↦w ∈ <[(i, r_t2) := WInt 0%Z]>
                (<[(i, r_t3) := WInt 0%Z]>
@@ -279,115 +545,143 @@ Section SimpleMalloc.
     iDestruct (big_sepM_delete _ _ (i, r_t8) with "Hrmap") as "[Hr8 Hrmap]".
     by rewrite !lookup_delete_ne //.
 
-  (* TODO move somewhere else *)
-  Tactic Notation "solve_length_seq" "by" tactic3(solve_a) :=
-    cbn ; try (rewrite finz_seq_between_length)
-    ; repeat (rewrite finz_dist_S ; last solve_a)
-    ; by rewrite finz_dist_0 ; last solve_a.
-
 
     (* Split the invariant into more fine-grained invariant *)
-    iDestruct (inv_split with "Hinv") as "[Hinv_code Hinv_lock]".
+    iDestruct (inv_split_l with "Hinv") as "Hinv_code".
     rewrite {2}/codefrag.
     rewrite {2}/malloc_subroutine_instrs /malloc_subroutine_instrs'.
-    rewrite (region_mapsto_split _ _ (b ^+ malloc_pre_spin_length)%a).
-    2:{ cbn; rewrite /malloc_pre_spin_length; solve_addr. }
-    2:{ cbn; rewrite /malloc_pre_spin_length.
-        assert (H0 : (b+8)%f = Some (b ^+8)%a) by solve_addr.
-        apply (finz_incr_iff_dist b (b ^+8)%a 8%nat) in H0.
-        destruct H0 as [_ ?].
-        symmetry. apply H0. }
-    rewrite (region_mapsto_split (b ^+ malloc_pre_spin_length)%a _
-               ((b ^+ malloc_pre_spin_length ^+ spinlock_length)%a)).
-    2:{ rewrite /malloc_pre_spin_length /spinlock_length; solve_addr. }
-    2:{ cbn; rewrite /malloc_pre_spin_length /spinlock_length.
-        set (b' := (b ^+ 8)%a).
-        assert (H0 : ((b ^+ 8)%a+6)%f = Some ((b ^+ 8)%a ^+6)%a) by solve_addr.
-        apply (finz_incr_iff_dist b' (b' ^+6)%a 6%nat) in H0.
-        destruct H0 as [_ ?].
-        symmetry. apply H0. }
-    iDestruct (inv_split with "Hinv_code") as "[Hinv_code_pre H']".
-    iDestruct (inv_split with "H'") as "[Hinv_code_spin Hinv_code_post]".
-    iClear "Hinv_code"; iClear "H'".
-    rewrite /length /=.
+    set ( b_spin := (b ^+ malloc_pre_length)%a ).
+    rewrite (region_mapsto_split _ _ b_spin).
+    2:{ cbn; subst b_spin ; rewrite /malloc_pre_length; solve_addr. }
+    2:{ cbn; subst b_spin ; rewrite /malloc_pre_length; solve_dist_finz. }
 
-    iAssert ( inv N (codefrag b (malloc_pre_spin e)))
-              as "Hinv_pre"  ; first iFrame "#".
-    iClear "Hinv_code_pre".
+    set ( b_post := (b_spin ^+ acquire_spinlock_length)%a ).
+    rewrite (region_mapsto_split b_spin _ b_post).
+    2:{ cbn ; subst b_spin b_post
+      ; rewrite /malloc_pre_length /acquire_spinlock_length; solve_addr. }
+    2:{ cbn ; subst b_spin b_post
+        ; rewrite /malloc_pre_length /acquire_spinlock_length
+        ; solve_dist_finz. }
 
-    iAssert ( inv N (codefrag (b ^+ malloc_pre_spin_length)%a
-                       (spinlock_instrs' r_t5 r_t6 r_t7 r_t8)))
-              as "Hinv_spin"  ; first iFrame "#".
-    iClear "Hinv_code_spin".
+    set ( b_release := (b_post ^+ malloc_post_length)%a ).
+    rewrite (region_mapsto_split b_post _ b_release).
+    2:{ cbn ; subst b_spin b_post b_release
+        ; rewrite /malloc_pre_length /acquire_spinlock_length /malloc_post_length
+        ; solve_addr. }
+    2:{ cbn ; subst b_spin b_post b_release
+        ; rewrite /malloc_pre_length /acquire_spinlock_length /malloc_post_length
+        ; solve_dist_finz. }
 
-    iAssert ( inv N (codefrag ((b ^+ malloc_pre_spin_length) ^+ spinlock_length)%a
-                       (malloc_post_spin (malloc_subroutine_instrs_length - (5 + spinlock_length)))))
+    set ( b_clear := (b_release ^+ 1)%a ).
+    rewrite (region_mapsto_split b_release _ b_clear).
+    2:{ cbn ; subst b_spin b_post b_release b_clear
+        ; rewrite /malloc_pre_length /acquire_spinlock_length /malloc_post_length
+        ; solve_addr. }
+    2:{ cbn ; subst b_spin b_post b_release b_clear
+        ; rewrite /malloc_pre_length /acquire_spinlock_length /malloc_post_length
+        ; solve_dist_finz. }
+    simpl.
+
+    iDestruct (inv_split with "Hinv_code") as "[Hinv_pre' H0]"
+    ; iClear "Hinv_code".
+    iDestruct (inv_split with "H0") as "[Hinv_spin' H1]"
+    ; iClear "H0".
+    iDestruct (inv_split with "H1") as "[Hinv_post' H2]"
+    ; iClear "H1".
+    iDestruct (inv_split with "H2") as "[Hinv_release' Hinv_clear']"
+    ; iClear "H2".
+
+    iAssert ( inv N (codefrag b (malloc_pre_spin offset_bm)))
+              as "Hinv_pre"
+    ; first iFrame "#"
+    ; iClear "Hinv_pre'".
+
+    iAssert ( inv N (codefrag b_spin
+                       (acquire_spinlock_instrs r_t5 r_t6 r_t7 r_t8)))
+              as "Hinv_spin"
+    ; first iFrame "#"
+    ; iClear "Hinv_spin'".
+
+    iAssert ( inv N (codefrag b_post
+                       (malloc_post_spin (offset_bm - malloc_pre_length - acquire_spinlock_length))))
               as "Hinv_post"
-    ; first ( iFrame "#"
-         ; rewrite /codefrag
-         ; simpl ; rewrite /malloc_pre_spin_length /malloc_pre_post_length /spinlock_length
-         ; replace ((((b ^+ 8) ^+ 6) ^+ 26%nat)%a) with (b ^+ 40%nat)%a by solve_addr
-         ; iFrame "#").
-    iClear "Hinv_code_post".
+    ; first iFrame "#"
+    ; iClear "Hinv_post'".
 
+
+    iAssert ( inv N (codefrag b_release (release_spinlock_instrs r_t5)))
+              as "Hinv_release"
+    ; first iFrame "#"
+    ; iClear "Hinv_release'".
+
+
+    iAssert ( inv N (codefrag b_clear malloc_clear))
+              as "Hinv_clear" ; [| iClear "Hinv_clear'"].
+    { iClear "Hinv".
+      iClear "Hinv_pre".
+      iClear "Hinv_post".
+      iClear "Hinv_spin".
+      iClear "Hinv_release".
+      rewrite /codefrag.
+      subst b_clear b_release b_post b_spin.
+      rewrite /malloc_pre_length /acquire_spinlock_length /malloc_post_length.
+      simpl.
+      replace (((((b ^+ 8) ^+ 6) ^+ 18) ^+ 1) ^+ 8%nat)%a
+        with ( b ^+ 41 )%a by solve_addr.
+      iFrame "#".
+    }
+    
     (** ====== Pre lock ====== *)
 
     iApply (wp_wand_l _ _ _ (λ v, ((φ v ∨ ⌜v = (i, FailedV)⌝) ∨ ⌜v = (i, FailedV)⌝)))%I. iSplitR.
     { iIntros (v) "[H|H] /=";auto. }
-    iApply (malloc_prelock_spec _ _ _ _ _ _ _ _ _ (fun v => (φ v ∨ ⌜v = (i, FailedV)⌝)%I)
-             with "[-$HPC $Hr1 $Hr2 $Hr3 $Hr5 Hinv_pre]") ;eauto.
+    iApply (malloc_prelock_spec _ _ _ _ _ _ _ _ _ _ _ (fun v => (φ v ∨ ⌜v = (i, FailedV)⌝)%I)
+             with "[-$HPC $Hr1 $Hr2 $Hr3 $Hr5]") ;eauto.
+    { rewrite /malloc_pre_length; solve_addr. }
     iSplitR.
-   { iClear "Hinv_lock"
-      ; iClear "Hinv_pre"
+   { (* We have to manipulate the invariant Hinv to extract the right one *)
+      iClear "Hinv_pre"
       ; iClear "Hinv_spin"
-      ; iClear "Hinv_post".
+      ; iClear "Hinv_post"
+      ; iClear "Hinv_release"
+      ; iClear "Hinv_clear".
 
-    (* iDestruct (inv_split with "Hinv") as "[Hinv_code Hinv_lock]". *)
-    rewrite {1}/codefrag.
-    rewrite {1}/malloc_subroutine_instrs /malloc_subroutine_instrs'.
-    rewrite (region_mapsto_split _ _ (b ^+ malloc_pre_spin_length)%a).
-    2:{ cbn; rewrite /malloc_pre_spin_length; solve_addr. }
-    2:{ cbn; rewrite /malloc_pre_spin_length.
-        assert (H' : (b+8)%f = Some (b ^+8)%a) by solve_addr.
-        apply (finz_incr_iff_dist b (b ^+8)%a 8%nat) in H'.
-        destruct H' as [_ H'].
-        symmetry; apply H'. }
-    rewrite (region_mapsto_split (b ^+ malloc_pre_spin_length)%a _
-               ((b ^+ malloc_pre_spin_length ^+ spinlock_length)%a)).
-    2:{ rewrite /malloc_pre_spin_length /spinlock_length; solve_addr. }
-    2:{ cbn; rewrite /malloc_pre_spin_length /spinlock_length.
-        set (b' := (b ^+ 8)%a).
-        assert (H' : ((b ^+ 8)%a+6)%f = Some ((b ^+ 8)%a ^+6)%a) by solve_addr.
-        apply (finz_incr_iff_dist b' (b' ^+6)%a 6%nat) in H'.
-        destruct H' as [_ H'].
-        symmetry; apply H'. }
-    match goal with
-    | h: _ |- context [ is_lock ?g ?b ?P] => set (L := is_lock g b P)
-    end.
-    match goal with
-    | h: _ |- context [ region_mapsto ?b ?e ?l ] => set (P1 := region_mapsto b e l)
-    end.
-    match goal with
-    | h: _ |- context [ region_mapsto ?b ?e ?l ] => set (P2 := region_mapsto b e l)
-    end.
-    match goal with
-    | h: _ |- context [ region_mapsto ?b ?e ?l ] => set (P3 := region_mapsto b e l)
-    end.
-    match goal with
-    | h: _ |- context [ mapsto ?e ?d ?v ] => set (IE := mapsto e d v)
-    end.
-    simpl.
-    iAssert ( inv N ( (P1 ∗ IE) ∗ ( P2 ∗ P3 ) ∗ L ) ) as "Hinv1".
-    iApply (inv_iff with "[$Hinv]")
-     ; first (do 2 iModIntro ; iSplit ;
-              [iIntros "((?&?&?) & ? & ?)" | iIntros "((? & ?) & (?&?) & ?)" ]
+      replace ( (b ^+ malloc_subroutine_instrs_length)%a )
+        with bm
+             by ( rewrite /malloc_subroutine_instrs_length; solve_addr).
+      rewrite {1}/codefrag.
+      rewrite {1}/malloc_subroutine_instrs /malloc_subroutine_instrs'.
+      rewrite (region_mapsto_split _ _ (b ^+ malloc_pre_length)%a).
+      2:{ cbn; rewrite /malloc_pre_length; solve_addr. }
+      2:{ cbn; rewrite /malloc_pre_length; solve_dist_finz. }
+      match goal with
+      | h: _ |- context [ is_lock ?g ?b ?P] => set (L := is_lock g b P)
+      end.
+      match goal with
+      | h: _ |- context [ mapsto ?e ?d ?v ] => set (IE := mapsto e d v)
+      end.
+      match goal with
+      | h: _ |- context [ ⌜?x1 = ?x2⌝%I ] => set (EQ := ⌜x1 = x2⌝%I)
+      end.
+      match goal with
+      | h: _ |- context [ region_mapsto ?b ?e ?l ] => set (P1 := region_mapsto b e l)
+      end.
+      match goal with
+      | h: _ |- context [ region_mapsto ?b ?e ?l ] => set (P2 := region_mapsto b e l)
+      end.
+
+      iAssert ( inv N ( (P1 ∗ IE) ∗ P2 ∗ EQ ∗ L ) ) as "Hinv1".
+      iApply (inv_iff with "[$Hinv]")
+      ; first (do 2 iModIntro ; iSplit ;
+               [iIntros "((?&?) & ? & ? & ?)" | iIntros "((? & ?) & ? & ? & ?)" ]
                ; iFrame).
-    iDestruct (inv_split_l with "Hinv1") as "Hinv2".
-    iClear "Hinv" ; iClear "Hinv1" ; clear -P1.
-    assert (P1 =  codefrag b (malloc_pre_spin e)).
-    { subst P1. rewrite /codefrag /malloc_pre_spin /malloc_pre_spin_length.
-      by cbn. }
-    auto.
+      iDestruct (inv_split_l with "Hinv1") as "Hinv2".
+      iClear "Hinv" ; iClear "Hinv1" ; clear -P1.
+      assert (P1 =  codefrag b (malloc_pre_spin offset_bm)).
+      { subst P1.
+        rewrite /codefrag /malloc_pre_spin /malloc_pre_length /offset_bm /= .
+        reflexivity. }
+      iFrame "Hinv2".
     }
     iNext ; iIntros "(HPC & Hr1 & Hr2 & Hr3 & Hr5 & %Hsize)".
     destruct Hsize as (size & ? & ->).
@@ -397,560 +691,246 @@ Section SimpleMalloc.
              "[-$HPC $Hr5 $Hr6 $Hr7 $Hr8]")
     ;[ apply ExecPCPerm_RX
        |.. ].
-    { rewrite /malloc_pre_spin_length ; solve_addr. }
+    { rewrite /malloc_pre_length ; solve_addr. }
     { auto. }
-    { admit. }
+    { solve_addr. }
     { eauto. }
     iSplitR.
-    { iAssert ( inv N (codefrag (b ^+ 8)%a (spinlock_instrs' r_t5 r_t6 r_t7 r_t8)
-                       ∗ is_lock γ (e ^+1)%a (∃ b_m a_m : Addr,
-                               ⌜(b + malloc_subroutine_instrs_length)%a = Some b_m⌝
-                                                                          ∗ b_m ↦ₐ WCap RWX b_m e a_m
-                                                                          ∗
-                                                                            [[a_m,e]]↦ₐ[[region_addrs_zeroes a_m e]] ∗ ⌜(b_m < a_m)%a ∧ (a_m <= e)%a⌝)))%I
-                as "Hinv_spinlock" .
-      admit.
-      iFrame "Hinv_spinlock". }
+    { (* we need to manipulate the invariant to get the right one *)
+      iClear "Hinv_pre"
+      ; iClear "Hinv_spin"
+      ; iClear "Hinv_post"
+      ; iClear "Hinv_clear"
+      ; iClear "Hinv_release".
+
+
+
+
+      replace ( (b ^+ malloc_subroutine_instrs_length)%a )
+        with bm
+             by ( rewrite /malloc_subroutine_instrs_length; solve_addr).
+
+    (* Split the invariant into more fine-grained invariant *)
+      clear b_clear b_release b_post b_spin.
+      iDestruct (inv_split_l with "Hinv") as "Hinv_code".
+      rewrite {1}/codefrag.
+      rewrite {1}/malloc_subroutine_instrs /malloc_subroutine_instrs'.
+      set ( b_spin := (b ^+ malloc_pre_length)%a ).
+      rewrite (region_mapsto_split _ _ b_spin).
+      2:{ cbn; subst b_spin ; rewrite /malloc_pre_length; solve_addr. }
+      2:{ cbn; subst b_spin ; rewrite /malloc_pre_length; solve_dist_finz. }
+
+      set ( b_post := (b_spin ^+ acquire_spinlock_length)%a ).
+      rewrite (region_mapsto_split b_spin _ b_post).
+      2:{ cbn ; subst b_spin b_post
+          ; rewrite /malloc_pre_length /acquire_spinlock_length; solve_addr. }
+      2:{ cbn ; subst b_spin b_post
+          ; rewrite /malloc_pre_length /acquire_spinlock_length
+          ; solve_dist_finz. }
+
+      match goal with
+      | h: _ |- context [ is_lock ?g ?b ?P] => set (L := is_lock g b P)
+      end.
+      match goal with
+      | h: _ |- context [ mapsto ?e ?d ?v ] => set (IE := mapsto e d v)
+      end.
+      match goal with
+      | h: _ |- context [ ⌜?x1 = ?x2⌝%I ] => set (EQ := ⌜x1 = x2⌝%I)
+      end.
+      match goal with
+      | h: _ |- context [ region_mapsto ?b ?e ?l ] => set (P1 := region_mapsto b e l)
+      end.
+      match goal with
+      | h: _ |- context [ region_mapsto ?b ?e ?l ] => set (P2 := region_mapsto b e l)
+      end.
+      match goal with
+      | h: _ |- context [ region_mapsto ?b ?e ?l ] => set (P3 := region_mapsto b e l)
+      end.
+
+
+      iAssert ( inv N ( (P2 ∗ L) ∗ (P1 ∗ P3) ∗ IE ∗ EQ ) ) as "Hinv1".
+      iApply (inv_iff with "[$Hinv]")
+      ; first (do 2 iModIntro ; iSplit ;
+               [iIntros "((?&?&?) & ? & ? & ?)"
+               | iIntros "((? & ?) & (?&?) & ? & ?)" ]
+               ; iFrame).
+      iDestruct (inv_split_l with "Hinv1") as "Hinv2".
+      iClear "Hinv" ; iClear "Hinv1" ; clear -P2.
+      assert (P2 =  codefrag (b ^+ malloc_pre_length)%a (acquire_spinlock_instrs r_t5 r_t6 r_t7 r_t8)).
+      { subst P2. rewrite /codefrag /acquire_spinlock_length /=.
+        done. }
+      rewrite H1.
+      iFrame "Hinv2".
+    }
+
     iNext ; iIntros "(HPC & Hr5 & Hr6 & Hr7 & Hr8 & Hbm & Hlocked)".
 
+
+
     (** ====== Post-Lock ======*)
+
     iDestruct "Hbm"
-      as (b_m a_m) "(%Hbm_bounds & Hb_m & Hfree_reg & %Ham_bounds)".
+      as (a_m) "(Hbm2 & Hmem & %Ham_bounds)".
     rewrite /length /=.
-    replace ( ((b ^+ malloc_pre_spin_length) ^+ 6%nat)%a )
+    replace ( ((b ^+ malloc_pre_length) ^+ 6%nat)%a )
       with (b ^+ 14)%a
-           by (rewrite /malloc_pre_spin_length ; solve_addr).
-    replace ( ((b ^+ malloc_pre_spin_length) ^+ spinlock_length)%a )
-      with (b ^+ 14)%a
-           by (rewrite /malloc_pre_spin_length /spinlock_length ; solve_addr).
+           by (rewrite /malloc_pre_length ; solve_addr).
+    replace (b ^+14)%a
+      with b_post
+           by
+           ( subst b_post b_spin
+             ; rewrite /malloc_pre_length /acquire_spinlock_length
+             ; solve_addr).
 
 
-    (* Mov *)
-    (* Open the invariant *)
-    wp_instr
-    ; iInv "Hinv_post" as ">Hprog" "Hcls"
-    (* Apply the invariant *)
-    ; iInstr_lookup "Hprog" as "Hi" "Hcont".
-    iApply ( wp_move_success_reg_fromPC with "[ $HPC $Hr2 $Hi ]") ; eauto.
-    { cbn ;rewrite decode_encode_instr_inv; eauto. }
-    { apply isCorrectPC_intro ; [solve_addr| auto]. }
-    { transitivity (Some ((b ^+ 14) ^+1)%a); solve_addr; done. }
-    iNext; iIntros "(HPC & Hi & Hr2)".
-    (* Close the invariant *)
-    iDestruct ("Hcont" with "Hi") as "Hprog".
-    iMod ("Hcls" with "Hprog") as "_".
-    simpl ; iModIntro ; wp_pure.
+    iApply ((malloc_postlock_spec i size b _ _ b_post a_m) with
+             "[-$HPC $Hr1 $Hr2 $Hr3 $Hr4]").
+    { subst b_post b_spin.
+      rewrite /malloc_pre_length /acquire_spinlock_length /malloc_post_length.
+      solve_addr. }
+    { subst b_post b_spin.
+      rewrite /malloc_pre_length /malloc_post_length /acquire_spinlock_length.
+      solve_addr. }
+    { eauto. }
+    replace (b ^+ (malloc_subroutine_instrs_length))%a
+      with bm by (rewrite /malloc_subroutine_instrs_length ; solve_addr).
 
-    (* Lea *)
-    (* Open the invariant *)
-    wp_instr
-    ; iInv "Hinv_post" as ">Hprog" "Hcls"
-    (* Apply the invariant *)
-    ; iInstr_lookup "Hprog" as "Hi" "Hcont".
-    iApply ( wp_lea_success_z with "[ $HPC $Hr2 $Hi ]") ; eauto.
-    { cbn ;rewrite decode_encode_instr_inv; eauto. }
-    { apply isCorrectPC_intro ; [solve_addr| auto]. }
-    { transitivity (Some ((b ^+ 14) ^+2)%a); solve_addr; done. }
-    { transitivity (Some (b ^+ 39)%a)
-      ; rewrite /spinlock_length /malloc_subroutine_instrs_length.
-      admit. done. } (* TODO correct the offset *)
-      (* ; solve_addr; done. } *)
-    iNext; iIntros "(HPC & Hi & Hr2)".
-    (* Close the invariant *)
-    iDestruct ("Hcont" with "Hi") as "Hprog".
-    iMod ("Hcls" with "Hprog") as "_".
-    simpl ; iModIntro ; wp_pure.
+    replace bm
+      with (b ^+ (malloc_subroutine_instrs_length))%a by
+           (rewrite /malloc_subroutine_instrs_length ; solve_addr).
+    rewrite /malloc_subroutine_instrs_length.
+    iFrame "Hbm2".
+    iFrame "Hinv_post".
 
-
-    (* Load *)
-    (* Open the invariant *)
-    replace (b ^+ 39)%a with b_m by admit.
-    (* by (rewrite /malloc_subroutine_instrs_length *)
-    (*                              in Hbm_bounds ; solve_addr). *)
-    wp_instr
-    ; iInv "Hinv_post" as ">Hprog" "Hcls"
-    (* Apply the invariant *)
-    ; iInstr_lookup "Hprog" as "Hi" "Hcont".
-    iApply ( wp_load_success_same_notinstr with "[ $HPC $Hr2 $Hi $Hb_m]") ; eauto.
-    { cbn ;rewrite decode_encode_instr_inv; eauto. }
-    { apply isCorrectPC_intro ; [solve_addr| auto]. }
-    { rewrite /malloc_subroutine_instrs_length in Hbm_bounds
-      ; solve_addr. }
-    { transitivity (Some ((b ^+ 14) ^+3)%a); solve_addr; done. }
-    iNext ; iIntros "(HPC & Hr2 & Hi & Hbm)".
-    (* Close the invariant *)
-    iDestruct ("Hcont" with "Hi") as "Hprog".
-    iMod ("Hcls" with "Hprog") as "_".
-    simpl ; iModIntro ; wp_pure.
-
-    (* GetA *)
-    (* Open the invariant *)
-    wp_instr
-    ; iInv "Hinv_post" as ">Hprog" "Hcls"
-    (* Apply the invariant *)
-    ; iInstr_lookup "Hprog" as "Hi" "Hcont".
-    iApply ( wp_Get_success with "[ $HPC $Hr3 $Hr2 $Hi ]") ; eauto.
-    { cbn ;rewrite decode_encode_instr_inv; eauto. }
-    { apply isCorrectPC_intro ; [solve_addr| auto]. }
-    { transitivity (Some ((b ^+ 14) ^+4)%a); solve_addr; done. }
-    iNext; iIntros "(HPC & Hi & Hr2 & Hr3)".
-    (* Close the invariant *)
-    iDestruct ("Hcont" with "Hi") as "Hprog".
-    iMod ("Hcls" with "Hprog") as "_".
-    simpl ; iModIntro ; wp_pure.
-    rewrite decode_encode_instr_inv /rules_Get.denote.
-
-
-    (* Lea might fail *)
-
-    (* Lea *)
-    (* Open the invariant *)
-    wp_instr
-    ; iInv "Hinv_post" as ">Hprog" "Hcls"
-    (* Apply the invariant *)
-    ; iInstr_lookup "Hprog" as "Hi" "Hcont".
-
-    destruct (a_m + size)%a as [a_m'|] eqn:Ha_m'; cycle 1.
-    { (* Failure case: no registered rule for that yet; do it the manual way *)
-      (* TODO: cf malloc, do not use rmap, but an empty map *)
-      iAssert ([∗ map] k↦x ∈ (∅:gmap (CoreN * RegName) Word), k ↦ᵣ x)%I as "-#Hregs".
-        by rewrite big_sepM_empty.
-
-      iDestruct (big_sepM_insert with "[$Hregs $Hr2]") as "Hregs".
-      by rewrite lookup_empty.
-      iDestruct (big_sepM_insert with "[$Hregs $Hr1]") as "Hregs".
-      rewrite !lookup_insert_ne
-      ; first by rewrite lookup_empty.
-      all: try (match goal with
-                | h:_ |- _ ≠ _ => simplify_pair_eq
-                end).
-      iDestruct (big_sepM_insert with "[$Hregs $HPC]") as "Hregs".
-      rewrite !lookup_insert_ne
-      ; first by rewrite lookup_empty.
-      all: try (match goal with
-                | h:_ |- _ ≠ _ => simplify_pair_eq
-                end).
-
-
-      iApply (wp_lea _ i RX b (e ^+2)%a ((b ^+ 14) ^+ 4)%a
-               with "[$Hregs $Hi]").
-      { rewrite decode_encode_instrW_inv; done. }
-      { admit. }
-      { apply lookup_insert. }
-      { rewrite /regs_of_core !dom_insert_L dom_empty_L. set_solver-. }
-      iNext. iIntros (regs' retv) "(Hspec & Hi & ?)".
-      iDestruct "Hspec" as %Hspec.
-
-      iDestruct ("Hcont" with "Hi") as "Hprog".
-      iMod ("Hcls" with "Hprog") as "_".
-
-      destruct Hspec as [| Hfail].
-      { exfalso.
-        clear - H4 Ha_m' H3 H1.
-        simplify_map_eq by simplify_pair_eq. }
-      { cbn.
-        iApply wp_pure_step_later; auto.
-        do 2 iModIntro.
-        iApply wp_value.
-        auto. } }
-
-
-
-    iApply ( wp_lea_success_reg with "[ $HPC $Hr2 $Hr1 $Hi ]") ; eauto.
-    { cbn ;rewrite decode_encode_instr_inv; eauto. }
-    { apply isCorrectPC_intro ; [solve_addr| auto]. }
-    { transitivity (Some ((b ^+ 14) ^+5)%a); solve_addr; done. }
-    iNext; iIntros "(HPC & Hi & Hr1 & Hr2)".
-    (* Close the invariant *)
-    iDestruct ("Hcont" with "Hi") as "Hprog".
-    iMod ("Hcls" with "Hprog") as "_".
-    simpl ; iModIntro ; wp_pure.
-
-    (* GetA *)
-    (* Open the invariant *)
-    wp_instr
-    ; iInv "Hinv_post" as ">Hprog" "Hcls"
-    (* Apply the invariant *)
-    ; iInstr_lookup "Hprog" as "Hi" "Hcont".
-    iApply ( wp_Get_success with "[ $HPC $Hr1 $Hr2 $Hi ]") ; eauto.
-    { cbn ;rewrite decode_encode_instr_inv; eauto. }
-    { apply isCorrectPC_intro ; [solve_addr| auto]. }
-    { transitivity (Some ((b ^+ 14) ^+6)%a); solve_addr; done. }
-    iNext; iIntros "(HPC & Hi & Hr2 & Hr1)".
-    (* Close the invariant *)
-    iDestruct ("Hcont" with "Hi") as "Hprog".
-    iMod ("Hcls" with "Hprog") as "_".
-    simpl ; iModIntro ; wp_pure.
-    rewrite decode_encode_instr_inv /rules_Get.denote.
-
-    (* Mov *)
-    (* Open the invariant *)
-    wp_instr
-    ; iInv "Hinv_post" as ">Hprog" "Hcls"
-    (* Apply the invariant *)
-    ; iInstr_lookup "Hprog" as "Hi" "Hcont".
-    iApply ( wp_move_success_reg with "[ $HPC $Hr4 $Hr2 $Hi ]") ; eauto.
-    { cbn ;rewrite decode_encode_instr_inv; eauto. }
-    { apply isCorrectPC_intro ; [solve_addr| auto]. }
-    { transitivity (Some ((b ^+ 14) ^+7)%a); solve_addr; done. }
-    iNext; iIntros "(HPC & Hi & Hr4 & Hr2)".
-    (* Close the invariant *)
-    iDestruct ("Hcont" with "Hi") as "Hprog".
-    iMod ("Hcls" with "Hprog") as "_".
-    simpl ; iModIntro ; wp_pure.
-    (* might fail *)
-    (* subseg *)
-    (* Open the invariant *)
-    wp_instr
-    ; iInv "Hinv_post" as ">Hprog" "Hcls"
-    (* Apply the invariant *)
-    ; iInstr_lookup "Hprog" as "Hi" "Hcont".
-
-    destruct (isWithin a_m a_m' b_m e) eqn:Ha_m'_within; cycle 1.
-    { (* Failure case: manual mode. *)
-      iAssert ([∗ map] k↦x ∈ (∅:gmap (CoreN * RegName) Word), k ↦ᵣ x)%I as "-#Hregs".
-        by rewrite big_sepM_empty.
-
-      iDestruct (big_sepM_insert with "[$Hregs $Hr4]") as "Hregs".
-      by rewrite lookup_empty.
-      iDestruct (big_sepM_insert with "[$Hregs $Hr3]") as "Hregs".
-      rewrite !lookup_insert_ne
-      ; first by rewrite lookup_empty.
-      all: try (match goal with
-                | h:_ |- _ ≠ _ => simplify_pair_eq
-                end).
-      iDestruct (big_sepM_insert with "[$Hregs $Hr1]") as "Hregs".
-      rewrite !lookup_insert_ne
-      ; first by rewrite lookup_empty.
-      all: try (match goal with
-                | h:_ |- _ ≠ _ => simplify_pair_eq
-                end).
-      iDestruct (big_sepM_insert with "[$Hregs $HPC]") as "Hregs".
-      rewrite !lookup_insert_ne
-      ; first by rewrite lookup_empty.
-      all: try (match goal with
-                | h:_ |- _ ≠ _ => simplify_pair_eq
-                end).
-
-      iApply (wp_Subseg with "[$Hregs $Hi]").
-      { rewrite decode_encode_instrW_inv; done. }
-      { admit. }
-      { apply lookup_insert. }
-      { rewrite /regs_of_core !dom_insert_L dom_empty_L. set_solver-. }
-      iNext. iIntros (regs' retv) "(Hspec & Hi & ?)".
-
-      iDestruct ("Hcont" with "Hi") as "Hprog".
-      iMod ("Hcls" with "Hprog") as "_".
-
-      iDestruct "Hspec" as %Hspec.
-      destruct Hspec as [| Hfail].
-      { exfalso. unfold addr_of_argument in *.
-        clear -H1 H3 H4 H5 Ha_m'_within.
-        simplify_map_eq by simplify_pair_eq.
-        repeat match goal with H:_ |- _ => apply finz_of_z_eq_inv in H end; subst.
-        congruence. }
-      { cbn. iModIntro. wp_pure. wp_end. auto. } }
-
-
-    
-    iApply ( wp_subseg_success with "[ $HPC $Hr4 $Hr3 $Hr1 $Hi ]") ; eauto.
-    { cbn ;rewrite decode_encode_instr_inv; eauto. }
-    { apply isCorrectPC_intro ; [solve_addr| auto]. }
-    { transitivity (Some a_m); solve_addr; done. }
-    { transitivity (Some (a_m ^+ size)%a); solve_addr; done. }
-    { transitivity (Some ((b ^+ 14) ^+8)%a); solve_addr; done. }
-    iNext; iIntros "(HPC & Hi & Hr3 & Hr1 & Hr4)".
-    (* Close the invariant *)
-    iDestruct ("Hcont" with "Hi") as "Hprog".
-    iMod ("Hcls" with "Hprog") as "_".
-    simpl ; iModIntro ; wp_pure.
-
-
-    (* sub *)
-    (* Open the invariant *)
-    wp_instr
-    ; iInv "Hinv_post" as ">Hprog" "Hcls"
-    (* Apply the invariant *)
-    ; iInstr_lookup "Hprog" as "Hi" "Hcont".
-    iApply ( wp_add_sub_lt_success_dst_r with "[ $HPC $Hr1 $Hr3 $Hi ]") ; eauto.
-    { rewrite decode_encode_instrW_inv ;cbn ; auto. }
-    { transitivity (Some ((b ^+ 14) ^+9)%a); solve_addr; done. }
-    { apply isCorrectPC_intro ; [solve_addr| auto]. }
-    iNext; iIntros "(HPC & Hi & Hr1 & Hr3)".
-    (* Close the invariant *)
-    iDestruct ("Hcont" with "Hi") as "Hprog".
-    iMod ("Hcls" with "Hprog") as "_".
-    simpl ; iModIntro ; wp_pure.
-    rewrite decode_encode_instr_inv /denote /=.
-    (* replace (a_m - (a_m ^+ size)%a)%Z with (-size)%Z by admit. *)
-
-    (* Lea *)
-    (* Open the invariant *)
-    wp_instr
-    ; iInv "Hinv_post" as ">Hprog" "Hcls"
-    (* Apply the invariant *)
-    ; iInstr_lookup "Hprog" as "Hi" "Hcont".
-    iApply ( wp_lea_success_reg with "[ $HPC $Hr4 $Hr3 $Hi ]") ; eauto.
-    { cbn ;rewrite decode_encode_instr_inv; eauto. }
-    { apply isCorrectPC_intro ; [solve_addr| auto]. }
-    { transitivity (Some ((b ^+ 14) ^+10)%a); solve_addr; done. }
-    { transitivity (Some a_m%a) ; solve_addr; done. }
-    iNext; iIntros "(HPC & Hi & Hr3 & Hr4)".
-    (* Close the invariant *)
-    iDestruct ("Hcont" with "Hi") as "Hprog".
-    iMod ("Hcls" with "Hprog") as "_".
-    simpl ; iModIntro ; wp_pure.
-
-    (* Mov *)
-    (* Open the invariant *)
-    wp_instr
-    ; iInv "Hinv_post" as ">Hprog" "Hcls"
-    (* Apply the invariant *)
-    ; iInstr_lookup "Hprog" as "Hi" "Hcont".
-    iApply ( wp_move_success_reg with "[ $HPC $Hr3 $Hr2 $Hi ]") ; eauto.
-    { cbn ;rewrite decode_encode_instr_inv; eauto. }
-    { apply isCorrectPC_intro ; [solve_addr| auto]. }
-    { transitivity (Some ((b ^+ 14) ^+11)%a); solve_addr; done. }
-    iNext; iIntros "(HPC & Hi & Hr3 & Hr2)".
-    (* Close the invariant *)
-    iDestruct ("Hcont" with "Hi") as "Hprog".
-    iMod ("Hcls" with "Hprog") as "_".
-    simpl ; iModIntro ; wp_pure.
-
-    (* sub *)
-    (* Open the invariant *)
-    wp_instr
-    ; iInv "Hinv_post" as ">Hprog" "Hcls"
-    (* Apply the invariant *)
-    ; iInstr_lookup "Hprog" as "Hi" "Hcont".
-    iApply ( wp_add_sub_lt_success_z_dst with "[ $HPC $Hr1 $Hi ]") ; eauto.
-    { rewrite decode_encode_instrW_inv ;cbn ; auto. }
-    { transitivity (Some ((b ^+ 14) ^+12)%a); solve_addr; done. }
-    { apply isCorrectPC_intro ; [solve_addr| auto]. }
-    iNext; iIntros "(HPC & Hi & Hr1)".
-    (* Close the invariant *)
-    iDestruct ("Hcont" with "Hi") as "Hprog".
-    iMod ("Hcls" with "Hprog") as "_".
-    simpl ; iModIntro ; wp_pure.
-    rewrite decode_encode_instr_inv /denote /=.
-    (* replace (a_m - (a_m ^+ size)%a)%Z with (-size)%Z by admit. *)
-
-
-    (* Lea *)
-    (* Open the invariant *)
-    wp_instr
-    ; iInv "Hinv_post" as ">Hprog" "Hcls"
-    (* Apply the invariant *)
-    ; iInstr_lookup "Hprog" as "Hi" "Hcont".
-    iApply ( wp_lea_success_reg with "[ $HPC $Hr3 $Hr1 $Hi ]") ; eauto.
-    { cbn ;rewrite decode_encode_instr_inv; eauto. }
-    { apply isCorrectPC_intro ; [solve_addr| auto]. }
-    { transitivity (Some ((b ^+ 14) ^+13)%a); solve_addr; done. }
-    { transitivity (Some 0%a) ; solve_addr; done. }
-    iNext; iIntros "(HPC & Hi & Hr1 & Hr3)".
-    (* Close the invariant *)
-    iDestruct ("Hcont" with "Hi") as "Hprog".
-    iMod ("Hcls" with "Hprog") as "_".
-    simpl ; iModIntro ; wp_pure.
-
-    (* GetB *)
-    (* Open the invariant *)
-    wp_instr
-    ; iInv "Hinv_post" as ">Hprog" "Hcls"
-    (* Apply the invariant *)
-    ; iInstr_lookup "Hprog" as "Hi" "Hcont".
-    iApply ( wp_Get_success with "[ $HPC $Hr1 $Hr3 $Hi ]") ; eauto.
-    { cbn ;rewrite decode_encode_instr_inv; eauto. }
-    { apply isCorrectPC_intro ; [solve_addr| auto]. }
-    { transitivity (Some ((b ^+ 14) ^+14)%a); solve_addr; done. }
-    iNext; iIntros "(HPC & Hi & Hr1 & Hr3)".
-    (* Close the invariant *)
-    iDestruct ("Hcont" with "Hi") as "Hprog".
-    iMod ("Hcls" with "Hprog") as "_".
-    simpl ; iModIntro ; wp_pure.
-    rewrite decode_encode_instr_inv /rules_Get.denote.
-
-
-    (* Lea *)
-    (* Open the invariant *)
-    wp_instr
-    ; iInv "Hinv_post" as ">Hprog" "Hcls"
-    (* Apply the invariant *)
-    ; iInstr_lookup "Hprog" as "Hi" "Hcont".
-    iApply ( wp_lea_success_reg with "[ $HPC $Hr3 $Hr1 $Hi ]") ; eauto.
-    { cbn ;rewrite decode_encode_instr_inv; eauto. }
-    { apply isCorrectPC_intro ; [solve_addr| auto]. }
-    { transitivity (Some ((b ^+ 14) ^+15)%a); solve_addr; done. }
-    { transitivity (Some b_m%a) ; solve_addr; done. }
-    iNext; iIntros "(HPC & Hi & Hr1 & Hr3)".
-    (* Close the invariant *)
-    iDestruct ("Hcont" with "Hi") as "Hprog".
-    iMod ("Hcls" with "Hprog") as "_".
-    simpl ; iModIntro ; wp_pure.
-
-    (* Store *)
-    (* Open the invariant *)
-    wp_instr
-    ; iInv "Hinv_post" as ">Hprog" "Hcls"
-    (* Apply the invariant *)
-    ; iInstr_lookup "Hprog" as "Hi" "Hcont".
-    iApply ( wp_store_success_reg with "[ $HPC $Hr2 $Hr3 $Hi $Hbm ]") ; eauto.
-    { cbn ;rewrite decode_encode_instr_inv; eauto. }
-    { apply isCorrectPC_intro ; [solve_addr| auto]. }
-    { transitivity (Some ((b ^+ 14) ^+16)%a); solve_addr; done. }
-    { solve_addr; done. }
-    iNext; iIntros "(HPC & Hi & Hr2 & Hr3 & Hbm)".
-    (* Close the invariant *)
-    iDestruct ("Hcont" with "Hi") as "Hprog".
-    iMod ("Hcls" with "Hprog") as "_".
-    simpl ; iModIntro ; wp_pure.
-
-    (* Mov *)
-    (* Open the invariant *)
-    wp_instr
-    ; iInv "Hinv_post" as ">Hprog" "Hcls"
-    (* Apply the invariant *)
-    ; iInstr_lookup "Hprog" as "Hi" "Hcont".
-    iApply ( wp_move_success_reg with "[ $HPC $Hr1 $Hr4 $Hi ]") ; eauto.
-    { cbn ;rewrite decode_encode_instr_inv; eauto. }
-    { apply isCorrectPC_intro ; [solve_addr| auto]. }
-    { transitivity (Some ((b ^+ 14) ^+17)%a); solve_addr; done. }
-    iNext; iIntros "(HPC & Hi & Hr1 & Hr4)".
-    (* Close the invariant *)
-    iDestruct ("Hcont" with "Hi") as "Hprog".
-    iMod ("Hcls" with "Hprog") as "_".
-    simpl ; iModIntro ; wp_pure.
+    iNext ; iIntros "(HPC & Hr1 & Hr2 & Hr3 & Hr4 & Hbm2 & %Hma')".
+    destruct Hma' as [a_m' Ha_m'].
 
     (** --- release the lock --- *)
+    destruct Ha_m' as [Ha_m' Ha_m'_bounds].
     rewrite (region_addrs_zeroes_split _ (a_m ^+ size)%a)
     ; [| solve_addr].
-    iDestruct (region_mapsto_split _ _ (a_m ^+ size)%a with "Hfree_reg")
+    iDestruct (region_mapsto_split _ _ (a_m ^+ size)%a with "Hmem")
       as "[Hmem_fresh Hmem]".
     solve_addr. by rewrite replicate_length //.
 
     iApply (release_spec i _ _ _ _ r_t5 _ _ _ _ _ (* define P ? *) N E γ _
              with "[-$HPC $Hlocked $Hr5]") ; auto.
     { apply ExecPCPerm_RX. }
+    { subst b_post b_spin ; rewrite /malloc_post_length /malloc_pre_length /acquire_spinlock_length.
+      solve_addr. }
     { solve_addr. }
-    { admit. }
     Unshelve.
-    2: { exact (∃ b_m0 a_m0 : Addr,
-               ⌜(b + malloc_subroutine_instrs_length)%a = Some b_m0⌝
-                                                          ∗ b_m0 ↦ₐ WCap RWX b_m0 e a_m0
-                                                          ∗ [[a_m0,e]]↦ₐ[[region_addrs_zeroes a_m0 e]] ∗ ⌜(b_m0 < a_m0)%a ∧ (a_m0 <= e)%a⌝)%I.
+    2: { exact (∃ a_m0 : Addr,
+                         ((b ^+ 41) ^+ 2)%a ↦ₐ WCap RWX (b ^+ 41)%a e a_m0
+                         ∗ [[a_m0,e]]↦ₐ[[region_addrs_zeroes a_m0 e]] ∗ ⌜((b ^+ 41) ^+ 2 < a_m0)%a ∧ (a_m0 <= e)%a⌝)%I.
     }
     iSplitR.
-    { iClear "Hinv_lock"
-      ; iClear "Hinv_pre"
+    { iClear "Hinv_pre"
       ; iClear "Hinv_spin"
-      ; iClear "Hinv_post".
+      ; iClear "Hinv_post"
+      ; iClear "Hinv_release"
+      ; iClear "Hinv_clear".
 
     (* iDestruct (inv_split with "Hinv") as "[Hinv_code Hinv_lock]". *)
-    rewrite {1}/codefrag.
-    rewrite {1}/malloc_subroutine_instrs /malloc_subroutine_instrs'.
-    rewrite (region_mapsto_split _ _ (b ^+ malloc_pre_spin_length)%a).
-    2:{ cbn; rewrite /malloc_pre_spin_length; solve_addr. }
-    2:{ cbn; rewrite /malloc_pre_spin_length.
-        assert (H' : (b+8)%f = Some (b ^+8)%a) by solve_addr.
-        apply (finz_incr_iff_dist b (b ^+8)%a 8%nat) in H'.
-        destruct H' as [_ H'].
-        symmetry; apply H'. }
-    rewrite (region_mapsto_split (b ^+ malloc_pre_spin_length)%a _
-               ((b ^+ malloc_pre_spin_length ^+ spinlock_length)%a)).
-    2:{ rewrite /malloc_pre_spin_length /spinlock_length; solve_addr. }
-    2:{ cbn; rewrite /malloc_pre_spin_length /spinlock_length.
-        set (b' := (b ^+ 8)%a).
-        assert (H' : ((b ^+ 8)%a+6)%f = Some ((b ^+ 8)%a ^+6)%a) by solve_addr.
-        apply (finz_incr_iff_dist b' (b' ^+6)%a 6%nat) in H'.
-        destruct H' as [_ H'].
-        symmetry; apply H'. }
-    match goal with
-    | h: _ |- context [ is_lock ?g ?b ?P] => set (L := is_lock g b P)
-    end.
-    match goal with
-    | h: _ |- context [ region_mapsto ?b ?e ?l ] => set (P1 := region_mapsto b e l)
-    end.
-    match goal with
-    | h: _ |- context [ region_mapsto ?b ?e ?l ] => set (P2 := region_mapsto b e l)
-    end.
-    match goal with
-    | h: _ |- context [ region_mapsto ?b ?e ?l ] => set (P3 := region_mapsto b e l)
-    end.
-    match goal with
-    | h: _ |- context [ mapsto ?e ?d ?v ] => set (IE := mapsto e d v)
-    end.
+    (* rewrite {1}/codefrag. *)
+    (* rewrite {1}/malloc_subroutine_instrs /malloc_subroutine_instrs'. *)
+    (* rewrite (region_mapsto_split _ _ (b ^+ malloc_pre_length)%a). *)
+    (* 2:{ cbn; rewrite /malloc_pre_length; solve_addr. } *)
+    (* 2:{ cbn; rewrite /malloc_pre_length ; solve_dist_finz. } *)
+    (* rewrite (region_mapsto_split (b ^+ malloc_pre_length)%a _ *)
+    (*            ((b ^+ malloc_pre_length ^+ spinlock_length)%a)). *)
+    (* 2:{ rewrite /malloc_pre_length /spinlock_length; solve_addr. } *)
+    (* 2:{ cbn; rewrite /malloc_pre_length /acquire_spinlock_length; solve_dist_finz. } *)
+    (* match goal with *)
+    (* | h: _ |- context [ is_lock ?g ?b ?P] => set (L := is_lock g b P) *)
+    (* end. *)
+    (* match goal with *)
+    (* | h: _ |- context [ region_mapsto ?b ?e ?l ] => set (P1 := region_mapsto b e l) *)
+    (* end. *)
+    (* match goal with *)
+    (* | h: _ |- context [ region_mapsto ?b ?e ?l ] => set (P2 := region_mapsto b e l) *)
+    (* end. *)
+    (* match goal with *)
+    (* | h: _ |- context [ region_mapsto ?b ?e ?l ] => set (P3 := region_mapsto b e l) *)
+    (* end. *)
+    (* match goal with *)
+    (* | h: _ |- context [ mapsto ?e ?d ?v ] => set (IE := mapsto e d v) *)
+    (* end. *)
 
-    subst P3. simpl.
-    replace (malloc_post_spin (malloc_subroutine_instrs_length - (5 + spinlock_length)))
-      with
-      (encodeInstrsW
-      [Mov r_t2 PC; Lea r_t2 (malloc_subroutine_instrs_length - (5 + spinlock_length))%Z;
-       Load r_t2 r_t2; GetA r_t3 r_t2; Lea r_t2 r_t1;
-       GetA r_t1 r_t2; Mov r_t4 r_t2; Subseg r_t4 r_t3 r_t1; Sub r_t3 r_t3 r_t1;
-       Lea r_t4 r_t3; Mov r_t3 r_t2; Sub r_t1 0%Z r_t1; Lea r_t3 r_t1; GetB r_t1 r_t3;
-       Lea r_t3 r_t1; Store r_t3 r_t2; Mov r_t1 r_t4]
-      ++ encodeInstrsW [Store r_t5 0]
-      ++
-      encodeInstrsW [Mov r_t2 0%Z;
-                     Mov r_t3 0%Z; Mov r_t4 0%Z; Mov r_t5 0%Z; Mov r_t6 0%Z; Mov r_t7 0%Z; Mov r_t8 0%Z;
-                     Jmp r_t0])
-    by (rewrite /malloc_post_spin ; auto).
-    rewrite (region_mapsto_split ((b ^+ malloc_pre_spin_length) ^+ spinlock_length)%a _
-               ((b ^+ 14) ^+ 17)%a ).
-    2:{ rewrite /malloc_pre_spin_length /spinlock_length; solve_addr. }
-    2:{ cbn; rewrite /malloc_pre_spin_length /spinlock_length.
-        replace ( ((b ^+ 8) ^+ 6)%a ) with ((b ^+ 14))%a by solve_addr.
-        set (b' := (b ^+ 14)%a).
-        assert (H' : ((b ^+ 14)%a+17)%f = Some ((b ^+ 14)%a ^+17)%a) by solve_addr.
-        apply (finz_incr_iff_dist b' (b' ^+17)%a 17%nat) in H'.
-        destruct H' as [_ H'].
-        symmetry; apply H'. }
+    (* subst P3. simpl. *)
+    (* replace (malloc_post_spin (malloc_subroutine_instrs_length - (5 + spinlock_length))) *)
+    (*   with *)
+    (*   (encodeInstrsW *)
+    (*   [Mov r_t2 PC; Lea r_t2 (malloc_subroutine_instrs_length - (5 + spinlock_length))%Z; *)
+    (*    Load r_t2 r_t2; GetA r_t3 r_t2; Lea r_t2 r_t1; *)
+    (*    GetA r_t1 r_t2; Mov r_t4 r_t2; Subseg r_t4 r_t3 r_t1; Sub r_t3 r_t3 r_t1; *)
+    (*    Lea r_t4 r_t3; Mov r_t3 r_t2; Sub r_t1 0%Z r_t1; Lea r_t3 r_t1; GetB r_t1 r_t3; *)
+    (*    Lea r_t3 r_t1; Store r_t3 r_t2; Mov r_t1 r_t4] *)
+    (*   ++ encodeInstrsW [Store r_t5 0] *)
+    (*   ++ *)
+    (*   encodeInstrsW [Mov r_t2 0%Z; *)
+    (*                  Mov r_t3 0%Z; Mov r_t4 0%Z; Mov r_t5 0%Z; Mov r_t6 0%Z; Mov r_t7 0%Z; Mov r_t8 0%Z; *)
+    (*                  Jmp r_t0]) *)
+    (* by (rewrite /malloc_post_spin ; auto). *)
+    (* rewrite (region_mapsto_split ((b ^+ malloc_pre_length) ^+ spinlock_length)%a _ *)
+    (*            ((b ^+ 14) ^+ 17)%a ). *)
+    (* 2:{ rewrite /malloc_pre_length /spinlock_length; solve_addr. } *)
+    (* 2:{ cbn; rewrite /malloc_pre_length /acquire_spinlock_length. *)
+    (*     replace ( ((b ^+ 8) ^+ 6)%a ) with ((b ^+ 14))%a by solve_addr. *)
+    (*     set (b' := (b ^+ 14)%a). *)
+    (*     assert (H' : ((b ^+ 14)%a+17)%f = Some ((b ^+ 14)%a ^+17)%a) by solve_addr. *)
+    (*     apply (finz_incr_iff_dist b' (b' ^+17)%a 17%nat) in H'. *)
+    (*     destruct H' as [_ H']. *)
+    (*     symmetry; apply H'. } *)
 
-    rewrite (region_mapsto_split ((b ^+ 14) ^+ 17)%a _
-               ((b ^+ 14) ^+ 18)%a ).
-    2:{ solve_addr. }
-    2:{ cbn.
-        replace ((b ^+ 14) ^+ 17)%a with ((b ^+ 31))%a by solve_addr.
-        replace ((b ^+ 14) ^+ 18)%a with ((b ^+ 31) ^+1)%a by solve_addr.
-        rewrite finz_dist_S ; last solve_addr.
-        rewrite finz_dist_0 ; last solve_addr.
-        done. }
-    match goal with
-    | h: _ |- context [ region_mapsto ?b ?e ?l ] => set (P3 := region_mapsto b e l)
-    end.
-    match goal with
-    | h: _ |- context [ region_mapsto ?b ?e ?l ] => set (P4 := region_mapsto b e l)
-    end.
-    match goal with
-    | h: _ |- context [ region_mapsto ?b ?e ?l ] => set (P5 := region_mapsto b e l)
-    end.
-    iAssert ( inv N ( (P4 ∗ L) ∗ (P1 ∗ P2 ∗ P3 ∗ P5) ∗ IE ) ) as "Hinv1".
-    iApply (inv_iff with "[$Hinv]")
-     ; first (do 2 iModIntro ; iSplit ;
-              [iIntros "((?&?&?&?&?) & ? & ?)" | iIntros "((? & ?) & (?&?&?&?) & ?)" ]
-               ; iFrame).
-    iDestruct (inv_split_l with "Hinv1") as "Hinv2".
-    iClear "Hinv" ; iClear "Hinv1" ; clear -P4.
-    assert (P4 =  codefrag ((b ^+ 14) ^+ 17)%a [encodeInstrW (Store r_t5 0)]).
-    { subst P4. rewrite /codefrag /=.
-      replace (((b ^+ 14) ^+ 17) ^+ 1%nat)%a with ((b ^+ 14) ^+ 18)%a by solve_addr.
-      done. }
-    rewrite H0.
-    iFrame "Hinv2".
+    (* rewrite (region_mapsto_split ((b ^+ 14) ^+ 17)%a _ *)
+    (*            ((b ^+ 14) ^+ 18)%a ). *)
+    (* 2:{ solve_addr. } *)
+    (* 2:{ cbn. *)
+    (*     replace ((b ^+ 14) ^+ 17)%a with ((b ^+ 31))%a by solve_addr. *)
+    (*     replace ((b ^+ 14) ^+ 18)%a with ((b ^+ 31) ^+1)%a by solve_addr. *)
+    (*     rewrite finz_dist_S ; last solve_addr. *)
+    (*     rewrite finz_dist_0 ; last solve_addr. *)
+    (*     done. } *)
+    (* match goal with *)
+    (* | h: _ |- context [ region_mapsto ?b ?e ?l ] => set (P3 := region_mapsto b e l) *)
+    (* end. *)
+    (* match goal with *)
+    (* | h: _ |- context [ region_mapsto ?b ?e ?l ] => set (P4 := region_mapsto b e l) *)
+    (* end. *)
+    (* match goal with *)
+    (* | h: _ |- context [ region_mapsto ?b ?e ?l ] => set (P5 := region_mapsto b e l) *)
+    (* end. *)
+    (* iAssert ( inv N ( (P4 ∗ L) ∗ (P1 ∗ P2 ∗ P3 ∗ P5) ∗ IE ) ) as "Hinv1". *)
+    (* iApply (inv_iff with "[$Hinv]") *)
+    (*  ; first (do 2 iModIntro ; iSplit ; *)
+    (*           [iIntros "((?&?&?&?&?) & ? & ?)" | iIntros "((? & ?) & (?&?&?&?) & ?)" ] *)
+    (*            ; iFrame). *)
+    (* iDestruct (inv_split_l with "Hinv1") as "Hinv2". *)
+    (* iClear "Hinv" ; iClear "Hinv1" ; clear -P4. *)
+    (* assert (P4 =  codefrag ((b ^+ 14) ^+ 17)%a [encodeInstrW (Store r_t5 0)]). *)
+    (* { subst P4. rewrite /codefrag /=. *)
+    (*   replace (((b ^+ 14) ^+ 17) ^+ 1%nat)%a with ((b ^+ 14) ^+ 18)%a by solve_addr. *)
+    (*   done. } *)
+    (* rewrite H0. *)
+    (* iFrame "Hinv2". *)
+      admit. (* TODO manipule with the invariant *)
     }
 
-    iSplitL "Hbm Hmem".
-    iExists b_m , (a_m^+size)%a.
+    iSplitL "Hbm2 Hmem".
+    iExists (a_m^+size)%a.
     replace a_m' with (a_m ^+size)%a by solve_addr.
     iFrame "∗%".
     iPureIntro. solve_addr.
     iNext; iIntros "(HPC & Hr5)".
-    replace (((b ^+ 14) ^+ 17) ^+ 1)%a with (((b ^+ 14) ^+ 18)%a) by solve_addr.
+    (* replace (((b ^+ 14) ^+ 17) ^+ 1)%a with (((b ^+ 14) ^+ 18)%a) by solve_addr. *)
+
+    (* TODO specification clear *)
 
     (* Mov *)
     (* Open the invariant *)
     wp_instr
-    ; iInv "Hinv_post" as ">Hprog" "Hcls"
+    ; iInv "Hinv_clear" as ">Hprog" "Hcls"
     (* Apply the invariant *)
     ; iInstr_lookup "Hprog" as "Hi" "Hcont".
     iApply ( wp_move_success_z with "[ $HPC $Hr2 $Hi ]") ; eauto.
